\let\negmedspace\undefined
\let\negthickspace\undefined
\documentclass[a4,12pt,onecolumn]{IEEEtran}
\usepackage{amsmath,amssymb,amsfonts,amsthm}
\usepackage{algorithmic}
\usepackage{graphicx}
\usepackage{textcomp}
\usepackage{xcolor}
\usepackage{txfonts}
\usepackage{listings}
\usepackage{enumitem}
\usepackage{mathtools}
\usepackage{gensymb}
\usepackage[breaklinks=true]{hyperref}
\usepackage{tkz-euclide}
\usepackage{listings}
\usepackage{circuitikz}
\usepackage{gvv}
\begin{document}
\title{
\Huge\textbf{ Discrete Assignment}\\
\Huge\textbf{EE1205} Signals and Systems\\
}
\author{Shravya Kantayapalam\\ EE23BTECH11030}
\maketitle
\textbf{Question} 

 If the sum of the first $ n $ terms of an AP is $4n - n^2$, what is the first term ($ S_1 $)? What is the sum of the first two terms? What is the second term? Similarly, find the 3rd, the 10th, and the $n$th terms.
 
\solution\\
\begin{table}[ht!]
\begin{center}
\begin{tabular}{|c|c|c|c|}
   \hline
   variable&value&description\\
   \hline 
   y(n)&$(4n-n^2)u(n)$& Sum of first n-terms\\
   \hline
   x(n)&-&$n^{th}$ term of the AP\\
   \hline 
   d&-&common difference of AP\\
   \hline
\end{tabular}
\caption{Table: Input Parameters}
\end{center}
\end{table}
\begin{align}
y\brak{n+1}&=\brak{4n-n^2}u\brak{n}
\end{align}
refer equation\eqref{eq:shift} ,equation \eqref{eq:11.9.5.26.2},equation \eqref{eq:11.9.5.26.3} from appendix
\begin{align}
z^{-1}Y\brak{z} &=4\brak{\frac{z^{-1}}{\brak{1-z^{-1}}^2}}-\frac{z^{-1}\brak{1+z^{-1}}}{\brak{1-z^{-1}}^3}\\
Y\brak{z} &=\frac{4}{\brak{1-z^{-1}}^2}-\frac{\brak{1+z^{-1}}}{\brak{1-z^{-1}}^3}\\
Y\brak{z}&=X\brak{z}U\brak{z}\\
X\brak{z}&=\frac{Y\brak{z}}{U\brak{z}}\\
X\brak{z}&=4\brak{\frac{1}{\brak{1-z^{-1}}}}-\frac{\brak{1+z^{-1}}}{\brak{1-z^{-1}}^2}\\
&=\frac{\brak{3-5z^{-1}}}{\brak{1-z^{-1}}^2}\\
&=\frac{3z}{z-1}-\frac{2z}{\brak{z-1}^2}
\end{align}
Using Contour Integration to find the inverse $Z$-transform,
\begin{align}
    x(n)&=\frac{1}{2\pi j}\oint_{C} X(z) \; z^{n-1} \; dz  \\
    &=\frac{1}{2\pi j}\oint_{C}\brak{\frac{3}{z-1}-\frac{2}{\brak{z-1}^2}}z^{n-1} \;dz \\
    R&=\frac{1}{\brak {m-1}!}\lim\limits_{z\to a}\frac{d^{m-1}}{dz^{m-1}}\brak {{(z-a)}^{m}f\brak z}  \\
    R&=R_1+R_2\\
    R_1&=\frac{1}{\brak {0}!}\lim\limits_{z\to 1}\frac{d^{0}}{dz^{0}}\brak {{(z-1)}\frac{3z^{n}}{z-1}}\\
    &=\lim\limits_{z\to 1}3z^{n}\\
    &=3\\
    R_2&=frac{1}{\brak {1}!}\lim\limits_{z\to 1}\frac{d}{dz}\brak{{(z-1)^2}\frac{-2z^{n}}{\brak{z-1}^2}}\\
    &=-\lim\limits_{z\to 1}\frac{d}{dz}\brak{2z^{n}}\\
    &=-\lim\limits_{z\to 1}2nz^{n-1}\\
    &=-2n\\
    R&= 3-2n\\
    x(n)&=(3-2n)u(n)\\
    \text{First term of AP x(0)} &=3\\
    \text{sum of first two terms is y(2)} &= 4(2) - (2)^2\\
    &=4\\
    \text{second term of AP x(1)}&=1\\
    \text{third term of AP x(2)}&=-1\\
    \text{tenth term of AP x(9)}&=-15\\
    \text{$n^{th}$ term of AP x(n)}&=(3-2n)u(n)
\end{align}
\end{document}
